rules1

theories/SLFRules.v
@@ -1,19 +1,509 @@
-(** * Reasoning Rules of Separation Logic *)
+(**
+
+Separation Logic Foundations
+
+Chapter: "Rules".
+
+Author: Arthur Charguéraud.
+License: MIT.
+
+*)
 
 Set Implicit Arguments.
-Require Import LibCore TLCbuffer Fmap.
-Require Import Semantics SepBase.
+From Sep Require Import SepBase.
+
+(** Implicit Types *)
+
+Implicit Types x f : var.
+Implicit Types b : bool.
+Implicit Types v : val.
+Implicit Types H : hprop.
+Implicit Types Q : val->hprop.
 
 
-(** * Structural rules *)
+(* ####################################################### *)
+(** * The chapter in a rush *)
 
-(** ** Rule of consequence *)
+(* ******************************************************* *)
+(** ** Structural rules *)
 
-(** ** Frame rule *)
+(** We have already introduced in the first two chapters all the
+    essential structural rules. *)
 
-(** ** Garbage collection rule *)
+(** The frame rule asserts that the precondition and the postcondition
+    can be extended together by an arbitrary heap predicate. *)
 
-(** ** Extraction rules *)
+Parameter triple_frame : forall t H Q H',
+  triple t H Q ->
+  triple t (H \* H') (Q \*+ H').
+
+(** The consequence rule enables to strengthen the precondition
+    and weaken the postcondition. *)
+
+Parameter triple_conseq : forall t H' Q' H Q,
+  triple t H' Q' ->
+  H ==> H' ->
+  Q' ===> Q ->
+  triple t H Q.
+
+(** The two extraction rules enable to extract pure facts and
+    existentially quantified variables from the precondition
+    into the Coq context. *)
+
+Parameter triple_hpure : forall t (P:Prop) H Q,
+  (P -> triple t H Q) ->
+  triple t (\[P] \* H) Q.
+Proof using. intros. applys* is_local_hpure. Qed.
+
+Parameter triple_hexists : forall t (A:Type) (J:A->hprop) Q,
+  (forall x, triple t (J x) Q) ->
+  triple t (hexists J) Q.
+
+(** The garbage collection rules enable to discard any desired
+    piece of heap from the precondition or the postcondition. 
+    (As we have seen, it is equivalent to state these two rules
+    by writing [H'] instead of [\Top].) *)
+
+Parameter triple_htop_pre : forall t H Q,
+  triple t H Q ->
+  triple t (H \* \Top) Q.
+
+Parameter triple_htop_post : forall t H Q,
+  triple t H (Q \*+ \Top) ->
+  triple t H Q.
+
+
+(* ******************************************************* *)
+(** ** Rules for terms *)
+
+(** In this chapter, for simplicity, we assume that all terms
+    are written in "A-normal form": the arguments of applications
+    and of conditionals are restricted to variables and value.
+    Such a requirement does not limit expressiveness.
+    For example, [if t0 then t1 else t2] can be encoded as 
+    [let x = t0 in if x then t1 else t2]. *)
+
+(** The reasoning rule for a sequence [t1;t2] resembles that of 
+    Hoare logic. The rule is:
+[[
+      {H} t1 {Q1}     {Q1 val_unit} t2 {Q}
+      -----------------------------------
+              {H} (t1;t2) {Q}
+]]
+    The application of [Q1] to [val_unit] is necessary because
+    [Q1] is the postcondition of [t1] so it has type [val->hprop], 
+    whereas the precondition of [t2] must have type [hprop].
+    By applying [Q1] to the expected result of [t1], which is
+    [val_unit] when [t1] has type [unit], we obtain the
+    expression [Q1 val_unit] which indeed has type [hprop]. *)
+
+Parameter triple_seq : forall t1 t2 H Q Q1,
+  triple t1 H Q1 ->
+  triple t2 (Q1 val_unit) Q ->
+  triple (trm_seq t1 t2) H Q.
+
+(** The reasoning rule for a let binding [let x = t1 in t2] could
+    be stated, in informal writing, in the form:
+[[
+      {H} t1 {Q1}     (forall x, {Q1 x} t2 {Q})
+      -----------------------------------------
+            {H} (let x = t1 in t2) {Q}
+]]
+  Yet, such a presentation makes a confusion between the [x] that
+  denotes a program variable in [let x = t1 in t2], and the [x]
+  that denotes a value when quantified as [forall x]. 
+  The correct statement involves a substitution from the variable
+  [x] to a value quantified as [forall v].
+[[
+      {H} t1 {Q1}     (forall v, {Q1 v} (subst x v t2) {Q})
+      -----------------------------------------------------
+                {H} (let x = t1 in t2) {Q}
+]]
+*)
+
+Parameter triple_let : forall x t1 t2 H Q Q1,
+  triple t1 H Q1 ->
+  (forall v, triple (subst x v t2) (Q1 v) Q) ->
+  triple (trm_let x t1 t2) H Q.
+
+(** The rule for a conditional is exactly like in Hoare logic.
+[[
+      b = true -> {H} t1 {Q}     b = false -> {H} t2 {Q}
+      --------------------------------------------------
+               {H} (if b then t1 in t2) {Q}
+]]
+*)
+
+Parameter triple_if_bool_case : forall b t1 t2 H Q,
+  (b = true -> triple t1 H Q) ->
+  (b = false -> triple t2 H Q) ->
+  triple (trm_if (val_bool b) t1 t2) H Q.
+
+(** The rule for a value [v] can be written as a triple with an
+    empty precondition and a postcondition asserting that the
+    result value [x] is equal to [v], in the empty heap.
+[[
+     ----------------------------
+      {\[]} v {fun v' => \[v' = v]}
+]]
+    Yet, it is more convenient in practice to work with a judgment
+    whose conclusion is of the form [{H}v{Q}], for an arbitrary
+    [H] and [Q]. For this reason, we prever the following rule for 
+    values:
+  
+      H ==> Q v
+      ---------
+      {H} v {Q}
+
+    It may not be completely obvious at first sight why this 
+    alternative rule is equivalent to the former. We will prove
+    the equivalence further in this chapter. *)
+
+Parameter triple_val : forall v H Q,
+  H ==> Q v ->
+  triple (trm_val v) H Q.
+
+(** A function definition [trm_fun x t1], expressed as a subterm in a 
+    program, evaluates to a value, more precisely to [val_fun x t1].
+    Again, we could consider a rule with an empty precondition:
+
+[[
+     ------------------------------------------------------
+      {\[]} (trm_fun x t1) {fun v' => \[v' = val_fun x t1]}
+]]
+   However, we prefer a conclusion of the form [{H}(trm_fun x t1){Q}].
+   We thus consider the following rule, very similar to [triple_val]:
+*)
+
+Parameter triple_fun : forall x t1 H Q,
+  H ==> Q (val_fun x t1) ->
+  triple (trm_fun x t1) H Q.
+
+(** Last but not least, we need a reasoning rule to reason about a
+    function application. Consider an application [(v1 v2)].
+    Assume [v1] to be a function, that is, to be of the form
+    [val_fun x t1]. Then, according to the beta-reduction rule,
+    the semantics of [(v1 v2)] is the same as that of [subst x v2 t1].
+    Thus, the triple [{H}(v1 v2){Q}] holds if the triple 
+    [{H}(subst x v2 t1){Q}] holds. This logic is captured by the
+    following rule. *)
+
+Lemma triple_app_fun : forall x v1 v2 t1 H Q,
+  v1 = val_fun x t1 ->
+  triple (subst x v2 t1) H Q ->
+  triple (trm_app v1 v2) H Q.
+
+(** The generalization to recursive functions is straightforward.
+    It is discussed further in this chapter. 
+    
+    The generalization to functions of several arguments follows
+    a similar pattern, although with a few additional technicalities.
+    N-ary functions and other language extensions such as records,
+    arrays, loops, data constructor and pattern matching are discussed
+    in the file [SLFExt.v]. *)
+
+
+(* ******************************************************* *)
+(** ** Specification of primitive operations *)
+
+Lemma triple_ref : forall v,
+  triple (val_ref v)
+    \[]
+    (fun r => \exists l, \[r = val_loc l] \* l ~~~> v).
+
+Lemma triple_get : forall v l,
+  triple (val_get (val_loc l))
+    (l ~~~> v)
+    (fun x => \[x = v] \* (l ~~~> v)).
+
+Lemma triple_set : forall w l v,
+  triple (val_set (val_loc l) w)
+    (l ~~~> v)
+    (fun r => \[r = val_unit] \* l ~~~> w).
+
+
+(* ####################################################### *)
+(** * The chapter in a rush *)
+
+(* ******************************************************* *)
+(** ** The combined structural rules *)
+
+(** The combined structural rule combines the consequence rule,
+    the frame rule, and the garbage collection rule into a 
+    single rule. The formulation eases the application of 
+    structural rules in many situations. *)
+
+(* EX1! (himpl_frame_l) *)
+(** Prove the combined structural rule. *)
+
+Lemma triple_conseq_frame_htop : forall H2 H1 Q1 t H Q,
+  triple t H1 Q1 ->
+  H ==> H1 \* H2 ->
+  Q1 \*+ H2 ===> Q \*+ \Top ->
+  triple t H Q.
+(* SOLUTION *)
+Proof using.
+
+Qed.
+(* /SOLUTION *)
+
+
+(* ******************************************************* *)
+(** ** Reasoning rules for recursive functions *)
+
+(** This reasoning rules for functions immediately generalizes 
+    to recursive functions. *)
+
+Parameter triple_fix : forall f x t1 H Q,
+  H ==> Q (val_fix f x t1) ->
+  triple (trm_fix f x t1) H Q.
+
+Lemma triple_app_fix : forall (f:bind) x F V t1 H Q,
+  F = (val_fix f x t1) ->
+  triple (subst2 f F x V t1) H Q ->
+  triple (trm_app F V) H Q.
+
+(** In fact, our language is set up in such a way that a non-recursive
+    function is just a special case of a (potentially-recursive) function.
+    The term [trm_fix z x t1] denotes a potentially-recursive function, 
+    where [z] is a binder. This binder may be either a variable [f],
+    in the case of a recursive function, or the special anonymous binder
+    written [bind_anon] to denote a non-recursive function. *)
+    
+Check trm_fix : bind -> var -> trm -> trm.
+
+Definition trm_fun x t1 := trm_fix bind_anon x t1.
+
+
+
+
+(* ******************************************************* *)
+(** ** Proofs for the rules for terms *)
+
+
+
+Lemma hoare_val : forall v H Q,
+  H ==> Q v ->
+  hoare (trm_val v) H Q.
+Proof using.
+  introv M. intros h Hh. exists h v. splits.
+  { applys red_val. }
+  { hhsimpl~. }
+Qed.
+
+Lemma hoare_fixs : forall (f:bind) xs t1 H Q,
+  xs <> nil ->
+  H ==> Q (val_fixs f xs t1) ->
+  hoare (trm_fixs f xs t1) H Q.
+Proof using.
+  introv N M. intros h Hh. exists___. splits.
+  { applys~ red_fixs. }
+  { hhsimpl~. }
+Qed.
+Lemma hoare_let : forall z t1 t2 H Q Q1,
+  hoare t1 H Q1 ->
+  (forall v, hoare (subst1 z v t2) (Q1 v) Q) ->
+  hoare (trm_let z t1 t2) H Q.
+Proof using.
+  introv M1 M2 Hh.
+  forwards* (h1'&v1&R1&K1): (rm M1).
+  forwards* (h2'&v2&R2&K2): (rm M2).
+  exists h2' v2. splits~. { applys~ red_let_trm R2. }
+Qed.Lemma hoare_if_bool : forall (b:bool) t1 t2 H Q,
+  hoare (if b then t1 else t2) H Q ->
+  hoare (trm_if b t1 t2) H Q.
+Proof using.
+  introv M1. intros h Hh. forwards* (h1'&v1&R1&K1): (rm M1).
+  exists h1' v1. splits~. { applys* red_if. }
+Qed.
+
+Lemma hoare_if_trm : forall Q1 t0 t1 t2 H Q, (* TODO needed? *)
+  hoare t0 H Q1 ->
+  (forall v, hoare (trm_if v t1 t2) (Q1 v) Q) ->
+  hoare (trm_if t0 t1 t2) H Q.
+Proof using.
+  introv M1 M2. applys* hoare_evalctx (fun t0 => trm_if t0 t1 t2).
+  { constructor. }
+Qed.
+Lemma hoare_apps_funs : forall xs F (Vs:vals) t1 H Q,
+  F = (val_funs xs t1) ->
+  var_funs (length Vs) xs ->
+  hoare (substn xs Vs t1) H Q ->
+  hoare (trm_apps F Vs) H Q.
+Proof using.
+  introv E N M. intros h Hh. forwards* (h'&v&R&K): (rm M).
+  exists h' v. splits~. { subst. applys* red_apps_funs. }
+Qed.
+
+Lemma triple_fun : forall x t1 H Q,
+  H ==> Q (val_fun x t1) ->
+  triple (trm_fun x t1) H Q.
+Proof using.
+  introv M. intros HF h N. exists___. splits.
+  { applys red_fun. }
+  { hhsimpl. hchanges M. }
+Qed.
+
+
+Lemma triple_val : forall v H Q,
+  H ==> Q v ->
+  triple (trm_val v) H Q.
+Proof using.
+  introv M. intros HF. applys hoare_val. { hchanges M. }
+Qed.
+
+Lemma triple_fixs : forall f xs t1 H Q,
+  xs <> nil ->
+  H ==> Q (val_fixs f xs t1) ->
+  triple (trm_fixs f xs t1) H Q.
+Proof using.
+  introv N M. intros HF. applys~ hoare_fixs. { hchanges M. }
+Qed.
+
+Lemma triple_constr : forall id vs H Q,
+  H ==> Q (val_constr id vs) ->
+  triple (trm_constr id vs) H Q.
+Proof using.
+  introv M. intros HF. applys hoare_constr. { hchanges M. }
+Qed.
+
+Lemma triple_constr_trm : forall id ts t1 vs H Q Q1,
+  triple t1 H Q1 -> 
+  (forall (X:val), triple (trm_constr id ((trms_vals vs)++(trm_val X)::ts)) (Q1 X) Q) ->
+  triple (trm_constr id ((trms_vals vs)++t1::ts)) H Q.
+Proof using.
+  introv M1 M2. intros HF. applys~ hoare_constr_trm.
+  { intros v. applys* hoare_of_triple. }
+Qed.
+
+Lemma triple_let : forall z t1 t2 H Q Q1,
+  triple t1 H Q1 ->
+  (forall (X:val), triple (subst1 z X t2) (Q1 X) Q) ->
+  triple (trm_let z t1 t2) H Q.
+Proof using.
+  introv M1 M2. intros HF. applys hoare_let.
+  { applys M1. }
+  { intros v. applys* hoare_of_triple. }
+Qed.
+
+Lemma triple_seq : forall t1 t2 H Q Q1,
+  triple t1 H Q1 ->
+  (forall (X:val), triple t2 (Q1 X) Q) ->
+  triple (trm_seq t1 t2) H Q.
+Proof using.
+  introv M1 M2. applys* triple_let. (* BIND intros. rewrite* subst1_anon. *)
+Qed.
+
+Lemma triple_if_bool : forall (b:bool) t1 t2 H Q,
+  triple (if b then t1 else t2) H Q ->
+  triple (trm_if b t1 t2) H Q.
+Proof using.
+  introv M1. intros HF. applys hoare_if_bool. applys M1.
+Qed.
+
+Lemma triple_if_bool_case : forall (b:bool) t1 t2 H Q,
+  (b = true -> triple t1 H Q) ->
+  (b = false -> triple t2 H Q) ->
+  triple (trm_if b t1 t2) H Q.
+Proof using.
+  introv M1 M2. applys triple_if_bool. case_if*.
+Qed.
+
+Lemma triple_if_trm : forall Q1 t0 t1 t2 H Q,
+  triple t0 H Q1 ->
+  (forall v, triple (trm_if v t1 t2) (Q1 v) Q) ->
+  triple (trm_if t0 t1 t2) H Q.
+Proof using.
+  introv M1 M2. intros HF. applys* hoare_if_trm.
+  { intros v. applys* hoare_of_triple. }
+Qed.
+
+Lemma triple_if : forall Q1 t0 t1 t2 H Q, (* not very useful *)
+  triple t0 H Q1 ->
+  (forall (b:bool), triple (if b then t1 else t2) (Q1 b) Q) ->
+  (forall v, ~ is_val_bool v -> (Q1 v) ==> \[False]) ->
+  triple (trm_if t0 t1 t2) H Q.
+Proof using.
+  introv M1 M2 M3. applys* triple_if_trm.
+  { intros v. tests C: (is_val_bool v).
+    { destruct C as (b&E). subst. applys* triple_if_bool. }
+    { xchange* M3. xpull ;=>. false. } }
+Qed.
+
+Lemma triple_apps_funs : forall xs F (Vs:vals) t1 H Q,
+  F = (val_funs xs t1) ->
+  var_funs (length Vs) xs ->
+  triple (substn xs Vs t1) H Q ->
+  triple (trm_apps F Vs) H Q.
+Proof using.
+  introv E N M. intros H' h Hf. forwards (h'&v&R&K): (rm M) Hf.
+  exists h' v. splits~. { subst. applys* red_apps_funs. }
+Qed.
+
+Lemma triple_apps_fixs : forall xs (f:var) F (Vs:vals) t1 H Q,
+  F = (val_fixs f xs t1) ->
+  var_fixs f (length Vs) xs ->
+  triple (substn (f::xs) (F::Vs) t1) H Q ->
+  triple (trm_apps F Vs) H Q.
+Proof using.
+  introv E N M. intros H' h Hf. forwards (h'&v&R&K): (rm M) Hf.
+  exists h' v. splits~. { subst. applys* red_apps_fixs. }
+Qed.
+
+
+(* ******************************************************* *)
+(** ** Proofs for the specification of primitive operations *)
+
+Lemma hoare_ref : forall H v,
+  hoare (val_ref v)
+    H
+    (fun r => (\exists l, \[r = val_loc l] \* l ~~~> v) \* H).
+Lemma hoare_get : forall H v l,
+  hoare (val_get (val_loc l))
+    ((l ~~~> v) \* H)
+    (fun x => \[x = v] \* (l ~~~> v) \* H).
+Proof using.
+  intros. intros h Hh. exists h v. splits~.
+  { applys red_get. destruct Hh as (h1&h2&(N1a&N1b)&N2&N3&N4).
+    subst h. applys~ fmap_union_single_l_read. }
+  { hhsimpl~. }
+Qed.
+
+Lemma hoare_set : forall H w l v,
+  hoare (val_set (val_loc l) w)
+    ((l ~~~> v) \* H)
+    (fun r => \[r = val_unit] \* (l ~~~> w) \* H).
+
+
+Lemma triple_ref : forall v,
+  triple (val_ref v)
+    \[]
+    (fun r => \exists l, \[r = val_loc l] \* l ~~~> v).
+Proof using.
+  intros. applys triple_of_hoare. intros HF. rew_heap.
+  esplit; split. { applys hoare_ref. } { hsimpl*. }
+Qed.
+
+Lemma triple_get : forall v l,
+  triple (val_get (val_loc l))
+    (l ~~~> v)
+    (fun x => \[x = v] \* (l ~~~> v)).
+Proof using.
+  intros. applys triple_of_hoare. intros HF.
+  esplit; split. { applys hoare_get. } { hsimpl*. }
+Qed.
+
+Lemma triple_set : forall w l v,
+  triple (val_set (val_loc l) w)
+    (l ~~~> v)
+    (fun r => \[r = val_unit] \* l ~~~> w).
+Proof using.
+  intros. applys triple_of_hoare. intros HF.
+  esplit; split. { applys hoare_set. } { hsimpl*. }
+Qed.
+
+
+
 
 
 (** * Rules for terms *)
