theories/SLFExt.v
@@ -1,0 +1,23 @@
+
+
+
+(* loops *)
+
+(* records *)
+
+(* arrays *)
+
+(* constr *)
+
+(* pattern *)
+
+(* not a-normal *)
+(** A conditional of the form [if t0 then t1 else t2] can
+    be encoded as [let x = t0 in if x then t1 else t2]. 
+    Thus, assuming programs to be written in A-normal form
+    (i.e., with arguments of conditionals and applications 
+    restricted to variables and values), one could live 
+    without a reasoning rule for [if t0 then t1 else t2].
+    Nevertheless, to support reasoning about programs that
+    are not written in A-normal form, we present more general
+    rules further in this chapter. *)
